\documentclass{article}
\usepackage[utf8]{inputenc}
\usepackage{geometry}
\usepackage{enumerate}
\usepackage{setspace}

\geometry{a4paper,scale=0.80}

\title{Number Theory (D)}
\author{}
\date{}

\begin{document}
	\begin{spacing}{1.5}
		\maketitle
		
		\section*{Prove:}
		Prove that $m = _{(_n)}p$ if and only if $m \% n=p\%n $.
		
		\subsection*{proof}
		I will prove that $m = _{(_n)}p$ if and only if $m \% n=p\%n $, by showing that 
		\begin{enumerate}[(a)]
			\item if $m = _{(_n)}p$, then $m \% n=p\%n $,
			\item if $m \% n=p\%n$, then $m = _{(_n)}p$.
		\end{enumerate}
		
		\subsubsection*{proof of (a)}
		By definition of \%,
		\begin{center}
			$ m \% n = m-(m \div n)n  $;\\
			$ p \% n = p-(p \div n)n  $.
		\end{center}
		Therefore, $ m \% n - p \% n = (m-p)-((m \div n)-(p \div n))n $.\\
		By definition of mod, if $ m = _{(_n)}p $, then $ n|(m-p) $.Plus, $ n|((m \div n)-(p \div n))n $.\\
		Therefore, $ n|(m \% n - p \% n) $. From fact, we know that $ 0 \leq m \% n < n $, so $ m \% n - p \% n $ can only be $ 0 $.\\
		Therefore, $m \% n=p\%n $.
		
		\subsubsection*{proof of (b)}
		Let $m\%n=p\%n=p'$,\\
		so $m=\lfloor \frac{m}{n}\rfloor n+p'$ and $p=\lfloor \frac{p}{n}\rfloor n+p'$.\\
		so $m-p=(\lfloor \frac{m}{n}\rfloor -\lfloor \frac{p}{n}\rfloor)n$.\\
		so $m=(\lfloor \frac{m}{n}\rfloor -\lfloor \frac{p}{n}\rfloor)n+p$.\\
		Therefore, $n|(m-p)$.\\
		Therefore, $m= _{(_n)}p$.\\
		Therefore,$m = _{(_n)}p$ if and only if $m \% n=p\%n $.
		
	\end{spacing}

	
	
\end{document}