\documentclass{article}
\usepackage[utf8]{inputenc}
\usepackage{geometry}
\usepackage{enumerate}
\usepackage{setspace}
\usepackage{amsmath}

\geometry{a4paper,scale=0.80}

\title{Set Theory (P)}
\author{}
\date{}

\begin{document}
	\begin{spacing}{1.5}
		\maketitle
		
		\section*{Prove:}
		Prove that for all sets $A \backslash (B \cup C) = (A \backslash B) \cap (A \backslash C)$.
		
		\subsection*{proof}
		\[
		\begin{array}{rclr}
			A \backslash (B \cup C) &=& A \cap (B \cap C)^{c} &\quad\text{(Definiton of $\backslash$)}\\
			&=& A \cap (B^{c} \cup C^{c}) &\quad\text{(de Morgan's Laws)}\\
			&=& A\cap A \cap (B^{c} \cap C^{c}) &\quad\text{(Idempotence of $ \cap $)}\\
			&=& A\cap (A \cap B^{c}) \cap C^{c} &\quad\text{(Associativity of $ \cap $)}\\
			&=& A\cap (B^{c} \cap A) \cap C^{c} &\quad\text{(Communitativity of $ \cap $)}\\
			&=& (A\cap B^{c}) \cap A \cap C^{c} &\quad\text{(Associativity of $ \cap $)}\\
			&=& (A\backslash B) \cap A \cap C^{c} &\quad\text{(Definiton of $\backslash$)}\\
			&=& (A\backslash B) \cap (A \backslash C) &\quad\text{(Definiton of $\backslash$)}\\
		\end{array}
		\]
	
		
	\end{spacing}
	
	
	
\end{document}